Define protocols in terms of projection/injection

src/Protocols.v
@@ -1,54 +1,118 @@
 Require Import CoopConcur.
 Require Import Automation.
+Require Import Equality.
 Import List.
 
-(** Generic structure defining a way to project some smaller set of
-state (memory and abstractions) Sigma' out of the global state Sigma.
+Section Protocols.
 
-The no_confusion well-formedness proofs guarantee Sigma' is actually
-less than or equal to Sigma. *)
-Record StateProj (Sigma:State) (Sigma': State) :=
-  defStateProj { memVars: variables (mem_types Sigma) (mem_types Sigma');
-                 abstractionVars: variables (abstraction_types Sigma) (abstraction_types Sigma');
-                 no_confusion_memVars : NoDup (hmap var_index memVars);
-                 no_confusion_abstractionVars : NoDup (hmap var_index abstractionVars) }.
+  Variables (Sigma Sigma':State).
 
-(** Generic proof that delta is a subprotocol of delta', both over the
-same global state.
+  (** Generic structure defining a way to project some smaller set of state
+      (memory and abstractions) Sigma' out of the global state Sigma.
 
-The subprotocol comes from the fact that valid states and transitions
-in delta are all valid in delta', so the state machine for delta is a
-subset of that for delta'. *)
-Definition SubProtocol (Sigma:State) (delta:Protocol Sigma) (delta':Protocol Sigma) :=
-  (forall d m s, invariant delta d m s -> invariant delta' d m s) /\
-  (forall tid s s', guar delta tid s s' -> guar delta' tid s s').
+      The no_confusion well-formedness proofs guarantee Sigma' is actually less
+      than or equal to Sigma. *)
+  Record StateProj :=
+    defStateProj { memVars: variables (mem_types Sigma) (mem_types Sigma');
+                   abstractionVars: variables (abstraction_types Sigma) (abstraction_types Sigma');
+                   no_confusion_memVars : NoDup (hmap var_index memVars);
+                   no_confusion_abstractionVars : NoDup (hmap var_index abstractionVars) }.
 
-Theorem rely_subprotocol : forall Sigma (delta delta': Protocol Sigma),
-    SubProtocol delta delta' ->
-    (forall tid s s', rely delta tid s s' -> rely delta' tid s s').
+  Variable (proj: StateProj).
+
+  (** * Projections into smaller state. *)
+
+  Definition pi__m (m: memory Sigma) : memory Sigma'.
+    destruct proj; unfold memory in *; simpl in *.
+    (* not relevant to the recursion *)
+    clear no_confusion_memVars0 no_confusion_abstractionVars0.
+    induction memVars0.
+    - apply HNil.
+    - apply HCons; hnf in *.
+      apply (Hlist.get b m).
+      apply IHmemVars0.
+  Defined.
+
+  Definition pi__s (m: abstraction Sigma) : abstraction Sigma'.
+    destruct proj; unfold abstraction in *; simpl in *.
+    clear no_confusion_memVars0 no_confusion_abstractionVars0.
+    induction abstractionVars0.
+    - apply HNil.
+    - apply HCons; hnf in *.
+      apply (Hlist.get b m).
+      apply IHabstractionVars0.
+  Defined.
+
+  (** Generic statement that a smaller delta' is a subprotocol of delta.
+
+      Transitions in delta correspond to transitions in delta', projected onto
+      Sigma'. *)
+  Definition SubProtocol delta delta' :=
+    (forall d m s, invariant delta d m s -> invariant delta' d (pi__m m) (pi__s s)) /\
+    (forall tid s s', guar delta tid s s' -> guar delta' tid (pi__s s) (pi__s s')).
+
+  Theorem rely_subprotocol : forall delta delta',
+      SubProtocol delta delta' ->
+      (forall tid s s', rely delta tid s s' -> rely delta' tid (pi__s s) (pi__s s')).
+  Proof.
+    unfold rely, others, SubProtocol; intuition.
+    induction H; try deex; eauto.
+  Qed.
+
+  (** * Injections into the global state. *)
+
+  (* TODO: factor out Hlist.set_all *)
+  Definition inj__m (m: memory Sigma) (m': memory Sigma') : memory Sigma.
+    destruct proj; unfold memory in *; simpl in *.
+    clear no_confusion_memVars0 no_confusion_abstractionVars0.
+    induction memVars0; hnf in *.
+    - exact m.
+    - eapply (Hlist.set b (get HFirst m')).
+      exact (IHmemVars0 (htail m')).
+  Defined.
+
+  Definition inj__s (s: abstraction Sigma) (s': abstraction Sigma') : abstraction Sigma.
+    destruct proj; unfold abstraction in *; simpl in *.
+    clear no_confusion_memVars0 no_confusion_abstractionVars0.
+    induction abstractionVars0; hnf in *.
+    - exact s.
+    - eapply (Hlist.set b (get HFirst s')).
+      exact (IHabstractionVars0 (htail s')).
+  Defined.
+
+  Definition InjectProtocol delta delta' :=
+    (forall d m s d' m' s', invariant delta d m s ->
+                       invariant delta' d' m' s' ->
+                       invariant delta d (inj__m m m') (inj__s s s')) /\
+    (forall tid s0 s s', guar delta' tid s s' ->
+                    guar delta tid (inj__s s0 s) (inj__s s0 s')).
+
+  Theorem rely_injectprotocol : forall delta delta',
+      InjectProtocol delta delta' ->
+      (forall tid s0 s s', rely delta' tid s s' ->
+                      rely delta tid (inj__s s0 s) (inj__s s0 s')).
+  Proof.
+    unfold rely, others, InjectProtocol; intuition.
+    induction H; try deex; eauto.
+  Qed.
+
+End Protocols.
+
+Theorem inj__m_get : forall Sigma Sigma' (proj: StateProj Sigma Sigma') m m'
+                       t (v_index: var (mem_types Sigma') t),
+    pi__m proj (inj__m proj m m') = m'.
 Proof.
-  unfold rely, others, SubProtocol; intuition.
-  induction H; try deex; eauto.
-Qed.
+  cbn; intros.
+  destruct proj; unfold memory in *; simpl.
+  induction memVars0; simpl.
+  - now inversion v_index.
+  - rewrite get_set.
+    apply hlist_get_extensional; intros.
+    dependent induction m0; cbn;
+      rewrite ?get_first, ?get_next;
+      eauto.
+Admitted.
 
-Record PrivateChanges Sigma PrivateSigma :=
-  { privateMemVars :
-      variables (mem_types Sigma) (mem_types PrivateSigma);
-    privateAbstractionVars :
-      variables (abstraction_types Sigma) (abstraction_types PrivateSigma) }.
-
-Definition privateVars {Sigma} {mtypes abstypes} memVars abstractionVars :=
-  Build_PrivateChanges Sigma (defState mtypes abstypes) memVars abstractionVars.
-
-Definition SubProtocolUnder Sigma PrivateSigma (private:PrivateChanges Sigma PrivateSigma)
-           (delta':Protocol Sigma) (delta:Protocol Sigma) :=
-  (forall d m s d' m' s',
-      invariant delta d m s ->
-      invariant delta' d m s ->
-      modified (privateMemVars private) m m' ->
-      modified (privateAbstractionVars private) s s' ->
-      invariant delta d' m' s') /\
-  (forall tid s s',
-      modified (privateAbstractionVars private) s s' ->
-      guar delta' tid s s' ->
-      guar delta tid s s').
+(* Local Variables: *)
+(* company-coq-local-symbols: (("delta" . ?δ) ("Sigma" . ?Σ)) *)
+(* End: *)
